a version of demo2

theory/x64Semantics.thy
@@ -67,7 +67,10 @@ fun x64_sem :: "nat \<Rightarrow> x64_bin \<Rightarrow> outcome \<Rightarrow> ou
 )"
 
 fun x64_sem1 :: "nat \<Rightarrow> u64 \<Rightarrow> (nat \<times> u64 \<times> x64_bin) list \<Rightarrow> outcome \<Rightarrow> outcome" where
-"x64_sem1 0 _ _ st = st" |
+"x64_sem1 0 _ _ st = (let st_temp = (
+  case st of
+    Next xpc rs m \<Rightarrow> Next 0 rs m |
+    Stuck \<Rightarrow> Stuck) in st_temp)" |
 "x64_sem1 (Suc n) pc lt xst = (
   let (num,off,l) = lt!(unat pc) in
   let xst_temp = (
@@ -77,6 +80,8 @@ fun x64_sem1 :: "nat \<Rightarrow> u64 \<Rightarrow> (nat \<times> u64 \<times> 
   let xst' = x64_sem num l xst_temp in (
     x64_sem1 n (pc+off) lt xst'))"
 
+
+value "x64_sem1 0 "
 
 (*definition x64_sem1 ::"nat \<Rightarrow> (nat \<times> x64_bin) list \<Rightarrow> outcome \<Rightarrow> outcome" where
 "x64_sem1 pc lt xst \<equiv> (let (fuel,l) = lt!pc in
